src/dafny/beacon/statetransition/StateTransition.s.dfy
@@ -23,6 +23,8 @@ include "../attestations/AttestationsTypes.dfy"
 include "../attestations/AttestationsHelpers.dfy"
 include "../Helpers.dfy"
 include "EpochProcessing.s.dfy"
+include "../forkchoice/ForkChoiceTypes.dfy"
+
 
 /**
  * State transition functional specification for the Beacon Chain.
@@ -40,6 +42,7 @@ module StateTransitionSpec {
     import opened BeaconHelpers
     import opened MathHelpers
     import opened EpochProcessingSpec
+    import opened ForkChoiceTypes
 
     /**
      *  Collect pubkey in a list of validators.
@@ -55,8 +58,6 @@ module StateTransitionSpec {
         else 
             { xv[0].pubkey } + keysInValidators(xv[1..])
     }
-
-   
 
     //  Specifications of finalisation of a state and forward to future slot.
 
@@ -94,12 +95,12 @@ module StateTransitionSpec {
     function addBlockToState(s: BeaconState, b: BeaconBlock) :  BeaconState 
         //  Verify that the slots match
         requires b.slot == s.slot  
-        // Verify that the parent matches
+        //  Verify that the parent matches
         requires b.parent_root == hash_tree_root(s.latest_block_header) 
         requires |s.validators| == |s.balances| 
         ensures |addBlockToState(s,b).validators| == |addBlockToState(s,b).balances|
         ensures addBlockToState(s,b).eth1_data_votes == s.eth1_data_votes
-        // ensures |addBlockToState(s,b).eth1_data_votes| == |s.eth1_data_votes|
+        //  ensures |addBlockToState(s,b).eth1_data_votes| == |s.eth1_data_votes|
         ensures addBlockToState(s,b).eth1_deposit_index == s.eth1_deposit_index
         ensures addBlockToState(s,b).validators == s.validators
         ensures addBlockToState(s,b).balances == s.balances
@@ -159,16 +160,16 @@ module StateTransitionSpec {
      *  @returns        A new state obtained by archiving roots and incrementing slot.
      *                  slot.
      */
-    function forwardStateToSlot(s: BeaconState, slot: Slot) : BeaconState 
+    function forwardStateToSlot(s: BeaconState, slot: Slot, store: Store) : BeaconState 
         requires s.slot <= slot
         requires |s.validators| == |s.balances|
 
-        ensures forwardStateToSlot(s, slot).slot == slot
-        ensures forwardStateToSlot(s, slot).eth1_deposit_index == s.eth1_deposit_index
-        ensures |forwardStateToSlot(s, slot).validators| == |forwardStateToSlot(s, slot).balances|
-        ensures forwardStateToSlot(s, slot).validators == s.validators
-        ensures forwardStateToSlot(s, slot).balances == s.balances
-        ensures forwardStateToSlot(s, slot).eth1_data_votes == s.eth1_data_votes
+        ensures forwardStateToSlot(s, slot, store).slot == slot
+        ensures forwardStateToSlot(s, slot, store).eth1_deposit_index == s.eth1_deposit_index
+        ensures |forwardStateToSlot(s, slot, store).validators| == |forwardStateToSlot(s, slot, store).balances|
+        ensures forwardStateToSlot(s, slot, store).validators == s.validators
+        ensures forwardStateToSlot(s, slot, store).balances == s.balances
+        ensures forwardStateToSlot(s, slot, store).eth1_data_votes == s.eth1_data_votes
         
         //  termination ranking function
         decreases slot - s.slot
@@ -176,7 +177,21 @@ module StateTransitionSpec {
         if (s.slot == slot) then 
             s
         else
-            nextSlot(forwardStateToSlot(s, slot - 1))
+            nextSlot(forwardStateToSlot(s, slot - 1, store), store)
+    }
+
+    lemma forwardStateIsNotStoreDependent(s: BeaconState, slot: Slot, store1: Store, store2: Store)
+        requires s.slot <= slot
+        requires |s.validators| == |s.balances|
+        ensures forwardStateToSlot(s, slot, store1) == forwardStateToSlot(s, slot, store2) 
+    {
+        if s.slot == slot {
+            //  Thanks Dafny 
+        } else {
+            var s' := forwardStateToSlot(s, slot - 1, store1);
+            forwardStateIsNotStoreDependent(s, slot - 1, store1, store2);
+            assert(nextSlot(s', store1) == nextSlot(s', store2));
+        }
     }
 
     /**
@@ -208,341 +223,36 @@ module StateTransitionSpec {
     /**
      *  Defines the value of state at next slot.
      */
-    function nextSlot(s: BeaconState) : BeaconState 
+    function nextSlot(s: BeaconState, store: Store) : BeaconState 
         requires s.slot as nat + 1 < 0x10000000000000000 as nat
         requires |s.validators| == |s.balances|
-        ensures nextSlot(s).latest_block_header.state_root != DEFAULT_BYTES32
+        ensures nextSlot(s, store).latest_block_header.state_root != DEFAULT_BYTES32
         /** If s.slot is not at the boundary of an epoch, the 
             attestation/finality fields are unchanged. */
         ensures  (s.slot as nat + 1) %  SLOTS_PER_EPOCH as nat != 0  ==>
-            nextSlot(s).justification_bits  == s.justification_bits
-            && nextSlot(s).previous_epoch_attestations  == s.previous_epoch_attestations
-            && nextSlot(s).current_epoch_attestations  == s.current_epoch_attestations
-            && nextSlot(s).previous_justified_checkpoint  == s.previous_justified_checkpoint
-            && nextSlot(s).current_justified_checkpoint  == s.current_justified_checkpoint
-            && nextSlot(s).validators  == s.validators
-            && nextSlot(s).balances  == s.balances
-            && |nextSlot(s).validators| == |nextSlot(s).balances| 
-            && nextSlot(s).eth1_data_votes ==  s.eth1_data_votes
-            &&  nextSlot(s).eth1_deposit_index  == s.eth1_deposit_index
-
+            nextSlot(s, store).justification_bits  == s.justification_bits
+            && nextSlot(s, store).previous_epoch_attestations  == s.previous_epoch_attestations
+            && nextSlot(s, store).current_epoch_attestations  == s.current_epoch_attestations
+            && nextSlot(s, store).previous_justified_checkpoint  == s.previous_justified_checkpoint
+            && nextSlot(s, store).current_justified_checkpoint  == s.current_justified_checkpoint
+            && nextSlot(s, store).validators  == s.validators
+            && nextSlot(s, store).balances  == s.balances
+            && |nextSlot(s, store).validators| == |nextSlot(s, store).balances| 
+            && nextSlot(s, store).eth1_data_votes ==  s.eth1_data_votes
+            &&  nextSlot(s, store).eth1_deposit_index  == s.eth1_deposit_index
     {
             if (s.slot + 1) %  SLOTS_PER_EPOCH == 0 then 
                 //  Apply update on partially resolved state, and then update slot
                 assert(s.slot % SLOTS_PER_EPOCH != 0);
                 // updateJustification(resolveStateRoot(s).(slot := s.slot)).(slot := s.slot + 1)
                 var s1 := resolveStateRoot(s).(slot := s.slot);
-                var s2 := updateJustificationAndFinalisation(s1);
-                var s3 := finalUpdates(s2);
+                var s2 := updateJustificationAndFinalisation(s1, store);
+                var s3 := finalUpdates(s2, store);
                 var s4 := s3.(slot := s.slot + 1);
                 s4
             else 
                 //  @note: this captures advanceSlot as a special case of resolveStateRoot 
                 resolveStateRoot(s)
     }
-
-    
-
-    /**
-     *  Simplified first-cut specification of process_justification_and_finalization.
-     *
-     *  @param  s   A beacon state the slot of which is not an Epoch boundary. 
-     *  @returns    The new state with justification checkpoints updated.
-     *  
-     */
-    // function updateJustificationPrevEpoch(s: BeaconState) : BeaconState 
-    //     /** State's slot is not an Epoch boundary. */
-    //     requires s.slot % SLOTS_PER_EPOCH != 0
-    //     /** Justification bit are right-shifted and last two are not modified.
-    //         Bit0 (new checkpoint) and Bit1 (previous checkpoint) may be modified.
-    //      */
-    //     ensures get_current_epoch(s) > GENESIS_EPOCH + 1 ==> 
-    //         updateJustificationPrevEpoch(s).justification_bits[2..] == 
-    //             (s.justification_bits)[1..|s.justification_bits| - 1]
-    // {
-    //     if  get_current_epoch(s) <= GENESIS_EPOCH + 1 then 
-    //         s 
-    //     else 
-    //         //  Right shift  justification_bits and prepend false
-    //         var newJustBits:= [false] + (s.justification_bits)[..JUSTIFICATION_BITS_LENGTH - 1];
-    //         //  Previous epoch checkpoint
-    //         //  Get attestations 
-    //         var matching_target_attestations := 
-    //             get_matching_target_attestations(s, get_previous_epoch(s));
-    //         var b1 := get_attesting_balance(s, matching_target_attestations) as nat * 3 
-    //                     >= get_total_active_balance(s) as nat * 2;
-    //         var c := CheckPoint(get_previous_epoch(s),
-    //                                     get_block_root(s, get_previous_epoch(s)));
-    //         s.(
-    //             current_justified_checkpoint := if b1 then c else s.current_justified_checkpoint,
-    //             previous_justified_checkpoint := s.current_justified_checkpoint,
-    //             justification_bits := if b1 then newJustBits[1 := true] else newJustBits
-    //         )
-    // }
-
-    // function updateJustification(s: BeaconState) : BeaconState
-    //     requires s.slot % SLOTS_PER_EPOCH != 0
-    //     // ensures updateJustification(s) == 
-    //     //     updateJustificationCurrentEpoch(updateJustificationPrevEpoch(s))
-    //     ensures get_current_epoch(s) > GENESIS_EPOCH + 1 ==> 
-    //         updateJustificationCurrentEpoch(s).justification_bits[1..] == 
-    //             (s.justification_bits)[1..|s.justification_bits|]
-    // {
-    //     updateJustificationCurrentEpoch(updateJustificationPrevEpoch(s))
-    // }
-
-    // function updateJustificationAndFinalisation(s: BeaconState) : BeaconState
-    //     requires s.slot % SLOTS_PER_EPOCH != 0
-    // {
-    //     updateFinalisedCheckpoint(updateJustification(s))
-    // }
-
-    // /**
-    //  *  Update related to the processing of current epoch.
-    //  */
-    // function updateJustificationCurrentEpoch(s: BeaconState) : BeaconState 
-    //     /** State's slot is not an Epoch boundary. */
-    //     requires s.slot % SLOTS_PER_EPOCH != 0
-    //     /** Justification bit are right-shifted and last two are not modified.
-    //         Bit0 (new checkpoint) and Bit1 (previous checkpoint) may be modified.
-    //      */
-    //     ensures get_current_epoch(s) > GENESIS_EPOCH + 1 ==> 
-    //         updateJustificationCurrentEpoch(s).justification_bits[1..] == 
-    //             (s.justification_bits)[1..|s.justification_bits|]
-    // {
-    //     if  get_current_epoch(s) <= GENESIS_EPOCH + 1 then 
-    //         s 
-    //     else 
-    //         //  Get attestations for current epoch
-    //         var matching_target_attestations := 
-    //             get_matching_target_attestations(s, get_current_epoch(s));
-    //         var b1 := get_attesting_balance(s, matching_target_attestations) as nat * 3 
-    //                     >= get_total_active_balance(s) as nat * 2;
-    //         var c := CheckPoint(get_current_epoch(s),
-    //                                     get_block_root(s, get_current_epoch(s)));
-    //         s.(
-    //             current_justified_checkpoint := if b1 then c else s.current_justified_checkpoint,
-    //             // previous_justified_checkpoint := s.current_justified_checkpoint,
-    //             justification_bits := if b1 then s.justification_bits[0 := true] else s.justification_bits
-    //         )
-    // }
-
-    // /**
-    //  *  Update a state finalised checkpoint.
-    //  *  @param  s   A state.
-    //  *  @returns    The new state after updating the status of finalised_checkpoint.
-    //  *  Epochs layout
-    //  *
-    //  *  | ............ | ........... | .......... | 
-    //  *  | ............ | ........... | .......... | 
-    //  *  e1             e2            e3           e4
-    //  *  bit[0]        bit[1]        bit[2]        bit[3]
-    //  *  current       previous
-    //  *
-    // //  *  Python slice a[k:l] means: a[k] ... a[l -1]
-    //  */
-    // function updateFinalisedCheckpoint(s: BeaconState) : BeaconState
-    //     ensures s.slot == updateFinalisedCheckpoint(s).slot
-    // {
-    //     if get_current_epoch(s) <= GENESIS_EPOCH + 1 then 
-    //         s 
-    //     else 
-    //         var bits : seq<bool> := s.justification_bits;
-    //         var current_epoch := get_current_epoch(s);
-    //         if (all(bits[1..4]) && current_epoch >= 3 && s.previous_justified_checkpoint.epoch  == current_epoch - 3) then 
-    //             //  The 2nd/3rd/4th most recent epochs are justified, the 2nd using the 4th as source
-    //             s.(finalised_checkpoint := s.previous_justified_checkpoint) 
-    //         else if (all(bits[1..3]) && s.previous_justified_checkpoint.epoch == current_epoch - 2) then 
-    //             // The 2nd/3rd most recent epochs are justified, the 2nd using the 3rd as source
-    //             s.(finalised_checkpoint := s.previous_justified_checkpoint) 
-    //         else if (all(bits[0..3]) && s.current_justified_checkpoint.epoch == current_epoch - 2) then 
-    //             // The 1st/2nd/3rd most recent epochs are justified, the 1st using the 3rd as source
-    //             s.(finalised_checkpoint := s.current_justified_checkpoint) 
-    //         else if (false && all(bits[0..2]) && s.current_justified_checkpoint.epoch == current_epoch - 1) then 
-    //             // The 1st/2nd most recent epochs are justified, the 1st using the 2nd as source
-    //             s.(finalised_checkpoint := s.current_justified_checkpoint) 
-    //         else
-    //             s 
-    // } 
-
-    // /**
-    //  *  Final section of process_final_updates where attestations are rotated.
-    //  *  @param  s   A beacon state.
-    //  *  @returns    `s` with the attestations rotated.
-    //  */
-    // function finalUpdates(s: BeaconState) : BeaconState
-    // {
-    //     s.(
-    //         previous_epoch_attestations := s.current_epoch_attestations,
-    //         current_epoch_attestations := []
-    //     )
-    // }
-
-
-
-    
-    // Helper lemmas
-
-
-    // lemma individualBalanceBoundMaintained(sb: seq<Gwei>, d: Deposit)
-    //     requires total_balances(sb) + d.data.amount as int < 0x10000000000000000
-    //     ensures forall i :: 0 <= i < |sb| ==> sb[i] as int + d.data.amount as int < 0x10000000000000000
-    // {
-    //     if |sb| == 0 {
-    //         // Thanks Dafny
-    //     }
-    //     else {
-    //         //assert total_balances(sb) == sb[0] as int + total_balances(sb[1..]);
-    //         //assert sb[0] as int + d.data.amount as int < 0x10000000000000000;
-    //         //assert total_balances(sb[1..]) + d.data.amount as int < 0x10000000000000000;
-    //         individualBalanceBoundMaintained(sb[1..],d);
-    //     }
-    // } 
-
-    // lemma updateBalTotalBySingleDeposit(s: BeaconState, d: Deposit)
-    //     requires s.eth1_deposit_index as int +  1 < 0x10000000000000000 
-    //     requires |s.validators| == |s.balances|
-    //     requires |s.validators| + 1 <= VALIDATOR_REGISTRY_LIMIT as int
-    //     requires total_balances(s.balances) + d.data.amount as int < 0x10000000000000000
-        
-    //     ensures total_balances(updateDeposit(s,d).balances) == total_balances(s.balances) + d.data.amount as int < 0x10000000000000000
-    //     //ensures total_balances(updateDeposit(s,d).balances) == total_balances(s.balances) + total_deposits([d]) 
-    // {
-    //     var pk := seqKeysInValidators(s.validators); 
-    //     if |s.balances| == 0 {
-    //         // Thanks Dafny
-    //     }
-    //     else {
-    //         if d.data.pubkey in pk {
-    //             var index := get_validator_index(pk, d.data.pubkey);
-    //             individualBalanceBoundMaintained(s.balances,d);
-    //             //assert updateDeposit(s,d).balances ==  increase_balance(s,index,d.data.amount).balances;
-    //             //assert increase_balance(s,index,d.data.amount).balances[index] == s.balances[index] + d.data.amount;
-    //             //assert forall i :: 0 <= i < |s.balances| && i != index as int ==> increase_balance(s,index,d.data.amount).balances[i] == s.balances[i];
-    //             //assert total_balances(updateDeposit(s,d).balances) == total_balances(increase_balance(s,index,d.data.amount).balances) ;
-    //             updateExistingBalance(s, index, d.data.amount);
-    //             //assert total_balances(updateDeposit(s,d).balances) == total_balances(s.balances) + d.data.amount as int ;
-    //         }
-    //         else {
-    //             //assert updateDeposit(s,d).balances == s.balances + [d.data.amount];
-    //             distBalancesProp(s.balances,[d.data.amount]);
-    //             //assert total_balances(s.balances + [d.data.amount]) == total_balances(s.balances) + total_balances([d.data.amount]);
-    //         }
-    //     }
-    // }
-
-    // lemma updateExistingBalance(s: BeaconState, index: ValidatorIndex, delta: Gwei)
-    //     requires index as int < |s.balances| 
-    //     requires s.balances[index] as int + delta as int < 0x10000000000000000
-    //     requires |s.balances| < VALIDATOR_REGISTRY_LIMIT as int
-
-    //     ensures total_balances(increase_balance(s,index,delta).balances) == total_balances(s.balances) + delta as int
-    // {
-    //     //assert increase_balance(s,index,delta).balances[index] == s.balances[index] + delta;
-    //     //assert forall i :: 0 <= i < |s.balances| && i != index as int ==> increase_balance(s,index,delta).balances[i] == s.balances[i];
-
-    //     if index as int < |s.balances|-1 {
-    //         assert increase_balance(s,index,delta).balances == increase_balance(s,index,delta).balances[..index] + [increase_balance(s,index,delta).balances[index]] + increase_balance(s,index,delta).balances[(index+1)..];
-                                                                
-    //         //assert total_balances(increase_balance(s,index,delta).balances[..index]) == total_balances(s.balances[..index]);
-    //         //assert total_balances([increase_balance(s,index,delta).balances[index]]) == total_balances([s.balances[index]]) + delta as int;
-    //         //assert total_balances(increase_balance(s,index,delta).balances[(index+1)..]) == total_balances(s.balances[(index+1)..]);
-
-    //         //assert total_balances(increase_balance(s,index,delta).balances) == total_balances(increase_balance(s,index,delta).balances[..index] + [increase_balance(s,index,delta).balances[index]] + increase_balance(s,index,delta).balances[(index+1)..]);
-
-    //         distBalancesProp(increase_balance(s,index,delta).balances[..index], [increase_balance(s,index,delta).balances[index]]);
-    //         //assert total_balances(increase_balance(s,index,delta).balances[..index] + [increase_balance(s,index,delta).balances[index]]) == total_balances(increase_balance(s,index,delta).balances[..index]) + total_balances([increase_balance(s,index,delta).balances[index]]);
-    //         distBalancesProp(increase_balance(s,index,delta).balances[..index]+[increase_balance(s,index,delta).balances[index]], increase_balance(s,index,delta).balances[(index+1)..]);
-    //         //assert total_balances(increase_balance(s,index,delta).balances[..index] + [increase_balance(s,index,delta).balances[index]] + increase_balance(s,index,delta).balances[(index+1)..]) == total_balances(increase_balance(s,index,delta).balances[..index]) + total_balances([increase_balance(s,index,delta).balances[index]]) + total_balances(increase_balance(s,index,delta).balances[index+1..]);
-
-    //         //assert total_balances(increase_balance(s,index,delta).balances) == total_balances(increase_balance(s,index,delta).balances[..index]) + total_balances([increase_balance(s,index,delta).balances[index]]) + total_balances(increase_balance(s,index,delta).balances[index+1..]);
-    //         //assert total_balances(increase_balance(s,index,delta).balances) == total_balances(s.balances[..index]) + total_balances([s.balances[index]]) + delta as int + total_balances(s.balances[(index+1)..]);
-
-    //         //assert total_balances(increase_balance(s,index,delta).balances) == total_balances(s.balances[..index]) + total_balances([s.balances[index]]) + total_balances(s.balances[(index+1)..]) + delta as int;
-
-    //         assert s.balances == s.balances[..index] + [s.balances[index]] + s.balances[(index+1)..];
-    //         //assert total_balances(s.balances) == total_balances(s.balances[..index] + [s.balances[index]] + s.balances[(index+1)..]);
-
-    //         distBalancesProp(s.balances[..index], [s.balances[index]]);
-    //         //assert total_balances(s.balances[..index] + [s.balances[index]]) == total_balances(s.balances[..index]) + total_balances([s.balances[index]]);
-    //         distBalancesProp(s.balances[..index]+[s.balances[index]], s.balances[(index+1)..]);
-    //         //assert total_balances(s.balances[..index] + [s.balances[index]] + s.balances[(index+1)..]) == total_balances(s.balances[..index]) + total_balances([s.balances[index]]) + total_balances(s.balances[index+1..]);
-
-    //         //assert total_balances(increase_balance(s,index,delta).balances) == total_balances(s.balances) + delta as int;
-    //     }
-    //     else {
-    //         //assert index as int == |s.balances| - 1;
-    //         assert increase_balance(s,index,delta).balances == increase_balance(s,index,delta).balances[..index] + [increase_balance(s,index,delta).balances[index]];
-                                                                
-    //         //assert total_balances(increase_balance(s,index,delta).balances[..index]) == total_balances(s.balances[..index]);
-    //         //assert total_balances([increase_balance(s,index,delta).balances[index]]) == total_balances([s.balances[index]]) + delta as int;
-            
-    //         //assert total_balances(increase_balance(s,index,delta).balances) == total_balances(increase_balance(s,index,delta).balances[..index] + [increase_balance(s,index,delta).balances[index]]);
-
-    //         distBalancesProp(increase_balance(s,index,delta).balances[..index], [increase_balance(s,index,delta).balances[index]]);
-    //         //assert total_balances(increase_balance(s,index,delta).balances[..index] + [increase_balance(s,index,delta).balances[index]]) == total_balances(increase_balance(s,index,delta).balances[..index]) + total_balances([increase_balance(s,index,delta).balances[index]]);
-            
-            
-    //         //assert total_balances(increase_balance(s,index,delta).balances) == total_balances(s.balances[..index]) + total_balances([s.balances[index]]) + delta as int;
-
-    //         assert s.balances == s.balances[..index] + [s.balances[index]] ;
-    //         //assert total_balances(s.balances) == total_balances(s.balances[..index] + [s.balances[index]]);
-
-    //         distBalancesProp(s.balances[..index], [s.balances[index]]);
-    //         //assert total_balances(s.balances[..index] + [s.balances[index]]) == total_balances(s.balances[..index]) + total_balances([s.balances[index]]);
-            
-    //         //assert total_balances(increase_balance(s,index,delta).balances) == total_balances(s.balances) + delta as int;
-    //     }
-    // }
-
-    // lemma distBalancesProp(sb1: seq<Gwei>, sb2: seq<Gwei>)
-    //     ensures total_balances(sb1 + sb2) == total_balances(sb1) + total_balances(sb2) 
-    // {
-    //     if |sb1| == 0 {
-    //         assert sb1 + sb2 == sb2;
-    //     }
-    //     else {
-    //         var sb := sb1 + sb2;
-    //         //assert sb == [sb1[0]] +  sb1[1..] + sb2;
-    //         assert sb[1..] == sb1[1..] + sb2;
-    //         assert total_balances(sb) == sb[0] as int + total_balances(sb[1..]);
-    //         //assert total_balances(sb1 + sb2) == sb[0] as int + total_balances(sb1[1..] + sb2);
-    //         distBalancesProp(sb1[1..],sb2);
-
-    //     }
-    // }
-
-    // lemma distDepositsProp(sd1: seq<Deposit>, sd2: seq<Deposit>)
-    //     ensures total_deposits(sd1 + sd2) == total_deposits(sd1) + total_deposits(sd2) 
-    // {
-    //     if |sd2| == 0 {
-    //         assert sd1 + sd2 == sd1;
-    //     }
-    //     else {
-    //         var sd := sd1 + sd2;
-    //         //assert sd == sd1 + sd2[..|sd2|-1] +  [sd2[|sd2|-1]];
-    //         assert sd[..|sd|-1] == sd1 + sd2[..|sd2|-1] ;
-    //         assert total_deposits(sd) == total_deposits(sd[..|sd|-1]) + sd2[|sd2|-1].data.amount as int;
-    //         //assert total_deposits(sd1 + sd2) == total_deposits(sd1 + sd2[..|sd2|-1] ) + sd2[|sd2|-1].data.amount as int;
-    //         distDepositsProp(sd1, sd2[..|sd2|-1] );
-    //     }
-    // }
-    // lemma subsetDepositSumProp(deposits: seq<Deposit>, i: nat)
-    //     requires i <= |deposits|
-    //     ensures total_deposits(deposits[..i]) <= total_deposits(deposits);
-    // {
-    //     if i == |deposits| {
-    //         assert deposits[..i] == deposits;
-    //     }
-    //     else {
-    //         //assert i < |deposits|;
-    //         assert deposits == deposits[..i] + deposits[i..];
-    //         assert total_deposits(deposits) == total_deposits(deposits[..i] + deposits[i..]);
-    //         distDepositsProp(deposits[..i], deposits[i..]);
-    //         //assert total_deposits(deposits[..i] + deposits[i..]) == total_deposits(deposits[..i]) + total_deposits(deposits[i..]); 
-    //     }
-    // }
-
-    
 
 }
